theories/rules/rules_Jmp.v
@@ -9,71 +9,113 @@ Section cap_lang_rules.
   Context `{MachineParameters}.
   Implicit Types P Q : iProp Σ.
   Implicit Types σ : ExecConf.
-  Implicit Types c : cap_lang.expr. 
+  Implicit Types c : cap_lang.expr.
   Implicit Types a b : Addr.
   Implicit Types r : RegName.
-  Implicit Types v : cap_lang.val. 
-  Implicit Types w : Word.
-  Implicit Types reg : gmap RegName Word.
-  Implicit Types ms : gmap Addr Word.
+  Implicit Types v : Version.
+  Implicit Types lw: LWord.
+  Implicit Types reg : Reg.
+  Implicit Types lregs : LReg.
+  Implicit Types mem : Mem.
+  Implicit Types lmem : LMem.
 
-  Lemma wp_jmp_success E pc_p pc_b pc_e pc_a w r w' :
-    decodeInstrW w = Jmp r →
-     isCorrectPC (WCap pc_p pc_b pc_e pc_a) →
+  Lemma wp_jmp_success E pc_p pc_b pc_e pc_a pc_v pca_v lw r lw' :
+    decodeInstrWL lw = Jmp r →
+     isCorrectLPC (LCap pc_p pc_b pc_e pc_a pc_v) →
 
-     {{{ ▷ PC ↦ᵣ WCap pc_p pc_b pc_e pc_a
-         ∗ ▷ pc_a ↦ₐ w
-         ∗ ▷ r ↦ᵣ w' }}}
+     {{{ ▷ PC ↦ᵣ LCap pc_p pc_b pc_e pc_a pc_v
+         ∗ ▷ (pc_a, pca_v) ↦ₐ lw
+         ∗ ▷ r ↦ᵣ lw' }}}
        Instr Executable @ E
        {{{ RET NextIV;
-           PC ↦ᵣ updatePcPerm w'
-           ∗ pc_a ↦ₐ w
-           ∗ r ↦ᵣ w' }}}.
+           PC ↦ᵣ updatePcPermL lw'
+           ∗ (pc_a, pca_v) ↦ₐ lw
+           ∗ r ↦ᵣ lw' }}}.
   Proof.
     iIntros (Hinstr Hvpc ϕ) "(>HPC & >Hpc_a & >Hr) Hφ".
+    apply isCorrectLPC_isCorrectPC_iff in Hvpc; cbn in Hvpc.
     iApply wp_lift_atomic_head_step_no_fork; auto.
     iIntros (σ1 ns l1 l2 nt) "Hσ1 /=". destruct σ1; simpl.
-    iDestruct "Hσ1" as "[Hr0 Hm]".
+    iDestruct "Hσ1" as (lr lm cur_map) "(Hr0 & Hm & %HLinv)"; simpl in HLinv.
     iDestruct (@gen_heap_valid with "Hm Hpc_a") as %?; auto.
     iDestruct (@gen_heap_valid with "Hr0 HPC") as %?.
     iDestruct (@gen_heap_valid with "Hr0 Hr") as %Hr_r0.
+    iDestruct (@gen_heap_valid with "Hr0 Hr") as %Hr_r0'.
     iModIntro. iSplitR. by iPureIntro; apply normal_always_head_reducible.
     iNext. iIntros (e2 σ2 efs Hpstep).
     apply prim_step_exec_inv in Hpstep as (-> & -> & (c & -> & Hstep)).
     iIntros "_".
     iSplitR; auto. eapply step_exec_inv in Hstep; eauto.
-    unfold exec, exec_opt in Hstep. rewrite Hr_r0 /= in Hstep. simplify_pair_eq.
+    2: eapply state_phys_log_reg_get_word in H3; eauto.
+    2: eapply state_phys_log_mem_get_word in H2; eauto.
+    unfold exec, exec_opt in Hstep; cbn in *.
+    eapply state_phys_log_reg_get_word in Hr_r0; eauto.
+    rewrite Hr_r0 /= in Hstep; simplify_pair_eq.
 
-    iMod (@gen_heap_update with "Hr0 HPC") as "[Hr0 HPC]". iFrame.
-    iApply "Hφ". by iFrame.
+    iMod (@gen_heap_update with "Hr0 HPC") as "[Hr0 HPC]".
+    iSplitR "Hφ HPC Hpc_a Hr" ; [|by iApply "Hφ" ; iFrame].
+    iExists _, lm, cur_map; iFrame; eauto; cbn.
+    iPureIntro; econstructor; eauto
+    ; [| by destruct HLinv as [_ ?]]
+    ; destruct HLinv as [[Hstrips Hcur_reg] HmemInv]
+    ; cbn in *.
+    rewrite -updatePcPermL_spec.
+    apply lreg_insert_respects_corresponds; [split ; auto|].
+    apply is_cur_updatePcPermL.
+    eapply lreg_read_iscur; eauto; split ; eauto.
   Qed.
 
-  Lemma wp_jmp_successPC E pc_p pc_b pc_e pc_a w :
-    decodeInstrW w = Jmp PC →
-     isCorrectPC (WCap pc_p pc_b pc_e pc_a) →
 
-     {{{ ▷ PC ↦ᵣ WCap pc_p pc_b pc_e pc_a
-         ∗ ▷ pc_a ↦ₐ w }}}
-       Instr Executable @ E
-       {{{ RET NextIV;
-           PC ↦ᵣ updatePcPerm (WCap pc_p pc_b pc_e pc_a)
-           ∗ pc_a ↦ₐ w }}}.
+  Lemma wp_jmp_successPC E pc_p pc_b pc_e pc_a pc_v pca_v lw :
+    decodeInstrWL lw = Jmp PC →
+    isCorrectLPC (LCap pc_p pc_b pc_e pc_a pc_v) →
+
+    {{{ ▷ PC ↦ᵣ LCap pc_p pc_b pc_e pc_a pc_v
+          ∗ ▷ (pc_a, pca_v) ↦ₐ lw }}}
+      Instr Executable @ E
+      {{{ RET NextIV;
+          PC ↦ᵣ updatePcPermL (LCap pc_p pc_b pc_e pc_a pc_v)
+            ∗ (pc_a, pca_v) ↦ₐ lw }}}.
   Proof.
     iIntros (Hinstr Hvpc ϕ) "(>HPC & >Hpc_a) Hφ".
+    apply isCorrectLPC_isCorrectPC_iff in Hvpc; cbn in Hvpc.
     iApply wp_lift_atomic_head_step_no_fork; auto.
-    iIntros (σ1 ns l1 l2 nt) "Hσ1 /=". destruct σ1; cbn.
-    iDestruct "Hσ1" as "[Hr0 Hm]".
+    iIntros (σ1 ns l1 l2 nt) "Hσ1 /=". destruct σ1; simpl.
+    iDestruct "Hσ1" as (lr lm cur_map) "(Hr0 & Hm & %HLinv)"; simpl in HLinv.
     iDestruct (@gen_heap_valid with "Hm Hpc_a") as %?; auto.
     iDestruct (@gen_heap_valid with "Hr0 HPC") as %Hr_PC.
+    iDestruct (@gen_heap_valid with "Hr0 HPC") as %Hr_PC'.
     iModIntro. iSplitR. by iPureIntro; apply normal_always_head_reducible.
     iNext. iIntros (e2 σ2 efs Hpstep).
     apply prim_step_exec_inv in Hpstep as (-> & -> & (c & -> & Hstep)).
     iIntros "_".
     iSplitR; auto. eapply step_exec_inv in Hstep; eauto.
-    unfold exec, exec_opt in Hstep. rewrite Hr_PC /= in Hstep. simplify_pair_eq.
+    2: eapply state_phys_log_reg_get_word in Hr_PC; eauto.
+    2: eapply state_phys_log_mem_get_word in H2; eauto.
+    unfold exec, exec_opt in Hstep; cbn in *.
+    eapply state_phys_log_reg_get_word in Hr_PC; eauto.
+    rewrite Hr_PC /= in Hstep; simplify_pair_eq.
 
-    iMod (@gen_heap_update with "Hr0 HPC") as "[Hr0 HPC]". iFrame.
-    iApply "Hφ". by iFrame.
+    iMod (@gen_heap_update with "Hr0 HPC") as "[Hr0 HPC]".
+    iSplitR "Hφ HPC Hpc_a" ; [|by iApply "Hφ" ; iFrame].
+    iExists _, lm, cur_map; iFrame; eauto; cbn.
+    iPureIntro; econstructor; eauto
+    ; [| by destruct HLinv as [_ ?]]
+    ; destruct HLinv as [[Hstrips Hcur_reg] HmemInv]
+    ; cbn in *.
+    replace (match pc_p with
+              | E => WCap RX pc_b pc_e pc_a
+              | _ => WCap pc_p pc_b pc_e pc_a
+              end)
+      with (lword_get_word (match pc_p with
+                            | E => LCap RX pc_b pc_e pc_a pc_v
+                            | _ => LCap pc_p pc_b pc_e pc_a pc_v
+                            end))
+           by (destruct pc_p ; auto).
+    apply lreg_insert_respects_corresponds ; [split ; auto|].
+    destruct pc_p; (try by eapply lreg_read_iscur; eauto; split ; eauto).
+    eapply is_cur_word_cap_change with (p':= machine_base.E) (a' := pc_a)
+    ; by eapply lreg_read_iscur; eauto; split ; eauto.
   Qed.
 
 End cap_lang_rules.
